# E(x)
![[Pasted image 20210129213524.png]]

Uniformly converges by Weierstrass M-test
![[Pasted image 20210129213548.png]]

# 3.27 Proposition
$\forall x,y \in \mathbb{R}, E(x+y)=E(x)E(y)$

### Proof
![[Pasted image 20210129213949.png]]

# 3.28 Corollary
![[Pasted image 20210129215441.png]]
![[Pasted image 20210129215448.png]]

### proof
- $E(x)>1+x$ => $\lim{E(x)}_{x\rightarrow + \infty}=+ \infty$
- $E(-x)=E(0)/E(x)=\frac {1}{E(x)}$ => $\lim{E(x)}_{x\rightarrow - \infty}=- \ \infty$

# 3.29 Proposition
$E(1)=e$

### proof
![[Pasted image 20210129220300.png]]
![[Pasted image 20210129220306.png]]
![[Pasted image 20210129220320.png]]

$E(x)=e^{x}$
$E^{-1}=log$ which is possible from [[3.2 Two Fundamental Theorems#^3d4d58| 3.16]] since it's always increasing it's continuous
- $\lim \limits_{x \rightarrow 0+} log(x) = - \infty$
- $\lim \limits_{x \rightarrow + \infty} log(x) = + \infty$

$b^{x}=e^{x \log{b}}$
$\log _{b} x = \log x / \log b$