# 4.6 Proposition
$\forall x \in \mathbb{R}: f(x)=x^n$ where $n\in \mathbb{Z}$ => $f$ is differentiable in $\mathbb{R}$ and $f'(x)=nx^{n-1}$

### proof
1. $n>1$ ($n=1,0$ are trivial)
$$
\begin{align}
f(y)-f(x)=y^n-x^n&=(y-x)(y^{n-1}+y^{n-2}+\dots +x^{n-1})=(y-x)\phi(y) \\
f'(x)&=\phi(x)=nx^{n-1}
\end{align}
$$

2. $n<0$
$$
\begin{align}
n<0 \Rightarrow \text{Let } n\in \mathbb{N}, \ f(x)&=x^{-n}\\
f(y)-f(x)&= \frac{x^n-y^n}{x^ny^n}=(y-x)\phi(y)\\
f'(x)&=\phi(x)=f'(x)=-nx^{-n-1}
\end{align}
$$

# 4.7 Proposition
$\forall x \in \mathbb{R}, \ E(x)=e^x$ => $E$ is differentiable in $\mathbb{R}$ and $E'=E$

### proof
$$
\begin{align}
\frac{E(x+h)-E(x)}{h}=E(x) \frac{E(h)-1}{h}\\
E(x)= \sum \limits _{n=0}^{\infty} \frac{x^n}{n!}\\
1+x< E(x) < 1+x+x^2\sum \limits_{n=1}^{\infty}\frac{1}{2^n}=1+x+x^2\\
x<E(x)-E(0)<x+x^2\\
1<\frac{E(h)-E(0)}{h}<1+h\\
\Rightarrow \lim \limits_{h \rightarrow 0^+}\frac{E(h)-E(0)}{h}=1
\end{align}
$$

