# 1.5.1 Definition (Partial Derivatives)
For the function $f(x,y)$
$$ \text{ Slope in x direction } = \left( \frac{\partial f}{\partial x} \right) _{y= \text{constant}} = \lim _{h \rightarrow 0} \left\{ \frac{f(x+h,y) - f(x,y)} {h} \right\}$$

# 1.5.1 Lemma (Partial derivative properties)
![[Pasted image 20210209145911.png]]
![[Pasted image 20210209145918.png]]
![[Pasted image 20210209145934.png]]

# 1.5.3 Alternative notation
## Partial derivative at a point
![[Pasted image 20210209150317.png]]

# 1.5.4 Definition (Partial derivatives in higher dimensions)
![[Pasted image 20210209150405.png]]

## 1.5.4.1 Lemma
All the properties before mentioned hold for higher dimension partial derivatives

# 1.5.5 Chain rule
Let $z=z(x)$ where $x=x(t)$
$$
\dfrac {dz}{dt} = \lim _{h \rightarrow 0} \frac{z(x(t+h))-z(x(t))} {h} = \lim _{h \rightarrow 0} \left( \frac {z(x(t+h))-z(x(t))} {x(t+h) - x(t)} \right) \left( \frac{x(t+h)-x(t)} {h} \right) = \frac {dz}{dx} \frac{dx}{dt}
$$
![[Pasted image 20210216213715.png]]

## 1.5.5.1 Note (Matrix multiplication representation)
![[Pasted image 20210216234510.png]]

# 1.5.7 Integration of Partial Derivatives

Let $z=f(x,y)$
$$ 
\int \left( \frac{\partial z}{\partial x} \right)_{y= \text{const}} dx = z(x,y)+g(y)
$$


To build the back the original equations you combine the two $\int \left( \frac{\partial z}{\partial x} \right) _{y= \text{const}}$ and $\int \left( \frac{\partial z}{\partial y} \right) _{x= \text{const}}$

## 1.5.7.1 Example 
![[Pasted image 20210217143359.png]]
![[Pasted image 20210217143407.png]]

## 1.5.7.2 Theorem  

$$ 
\frac{\partial u}{\partial x} (x,y) = \frac{\partial u}{\partial y} = 0
$$
$u(x,y)$ is constant on $\mathbb{R}^2$

# 1.5.8 Chain rule in First Order PDEs
$$
\frac {\partial z}{\partial t} + c \frac{\partial z}{\partial x} =  0 
$$

$$
\begin{align}
&\text{Let } \xi = x -ct \quad \eta = x + ct \\
&\text{so that } z(x,t)=z(x( \xi , \eta ), t( \xi , \eta ))= z( \xi , \eta ) \\
\end{align}
$$

$$
\begin{aligned}
\frac{\partial z}{\partial t} &= \frac{\partial \xi}{\partial t} \frac{\partial z}{\partial \xi} + \frac{\partial \eta}{\partial t} \frac{\partial z}{\partial \eta} = -c \frac{d z}{d \xi}+c \frac{dz}{d \eta} \\
\frac{\partial z}{\partial x} &= \frac{\partial \xi}{\partial x} \frac{\partial z}{\partial \xi} + \frac{\partial \eta}{\partial x} \frac{\partial z}{\partial \eta}= \frac{d z}{d \xi}+ \frac{dz}{d \eta} \\
\end{aligned}
$$

$$
\begin{align}
\frac {\partial z}{\partial t} + c \frac{\partial z}{\partial x}=2c \frac{\partial z}{\partial \eta}=0 \\
\frac {\partial z}{\partial \eta} = 0\\
\Rightarrow z=F(\xi) \\
z(x,t)=F(x-ct) \\
\end{align}
$$

# 1.5.9 Definition (Jacobian Matrix and Chain rule)

Let $f$ be a vector function: $f: (x,y) \rightarrow (f_1(x,y),f_2(x,y))$
could be represented $f(x,y)=f_1(x,y) \mathbf{i}+f_2(x,y) \mathbf{j}$

$$
J_f(x,y)=
\begin{pmatrix}
\frac{\partial f_1}{\partial x} & \frac{\partial f_1}{\partial y} \\
\frac{\partial f_2}{\partial x} & \frac{\partial f_2}{\partial y}
\end{pmatrix}
$$

define $g: (x,y) \rightarrow (x(s,t), y(s,t))$

$$
\begin{align}

\begin{pmatrix}
\frac{\partial f_1}{\partial s} & \frac{\partial f_1}{\partial t}
\end{pmatrix}
&=
\begin{pmatrix}
\frac{\partial f_1}{\partial x} & \frac{\partial f_`}{\partial y}
\end{pmatrix}

\begin{pmatrix}
\frac{\partial x}{\partial s} & \frac{\partial x}{\partial t} \\
\frac{\partial y}{\partial s} & \frac{\partial y}{\partial t}
\end{pmatrix}\\

\begin{pmatrix}
\frac{\partial f_2}{\partial s} & \frac{\partial f_2}{\partial t}
\end{pmatrix}
&=
\begin{pmatrix}
\frac{\partial f_2}{\partial x} & \frac{\partial f_2}{\partial y}
\end{pmatrix}

\begin{pmatrix}
\frac{\partial x}{\partial s} & \frac{\partial x}{\partial t} \\
\frac{\partial y}{\partial s} & \frac{\partial y}{\partial t}
\end{pmatrix}\Rightarrow \\

\begin{pmatrix}
\frac{\partial f_1}{\partial s} & \frac{\partial f_1}{\partial t}\\
\frac{\partial f_2}{\partial s} & \frac{\partial f_2}{\partial t}
\end{pmatrix}
&=
\begin{pmatrix}
\frac{\partial f_1}{\partial x} & \frac{\partial f_1}{\partial y}\\
\frac{\partial f_2}{\partial x} & \frac{\partial f_2}{\partial y}
\end{pmatrix}

\begin{pmatrix}
\frac{\partial x}{\partial s} & \frac{\partial x}{\partial t} \\
\frac{\partial y}{\partial s} & \frac{\partial y}{\partial t}
\end{pmatrix}\\

\end{align}
$$

$$
\begin{align}
\mathbb{R}^2_{(x,y)} \xrightarrow{g} \mathbb{R}^2_{(s,t)} \xrightarrow{f} \mathbb{R}^2 \\
J_{f \circ g}(s,t)=J_f (x,y) J_g (s,t)
\end{align}
$$

# 1.5.9.6 Theorem (chain rule)
$G : \mathbb{R}^m \rightarrow \mathbb{R}^n$ and $F : \mathbb{R}^n \rightarrow \mathbb{R}^p$, $G$ is diff. at $a$ and $F$ is diff at $b=G(a)$

$$
J_{F \circ G}(a)=J_F(b) \cdot J_G(a)
$$
![[Pasted image 20210222220707.png]]


# 1.5.9.6.1 Definition (Jacobian determinant)
$$
\det{J_f}= \frac{\partial(f_1 \dots f_n)}{\partial  (x_1 \dots x_n)}
$$

# 1.5.9.7 Theorem (inverse $f$, implicit $f$ theorem)
$f_1(x,y)$ and $f_2(x,y)$ are diff at $P:(x,y)=(a,b)$ and $\frac{\partial (f_1,f_2)}{\partial(x,y)} | _P  \neq 0$
=>
$\exists x(f_1,f_2)=x$ and $\exists y(f_1,f_2)=y$



