## 1.6.1 Example (implicit differentiation of x,y)

Given $F(x,y)=0$ find $\frac{dy}{dx}$

$$
\begin{align}
F(x,y)=F(x,y(x))=0 \\
\frac{\partial F}{\partial x} + \frac{\partial F}{\partial y} \frac{\partial y}{\partial x} = 0 \\
\frac{dy}{dx}=-\frac{\partial F}{\partial x} / \frac{\partial F}{\partial y}\\
\end{align}
$$

#### Example
Consider $F(x,y)=x^2+y^2-1=0$

$$
\begin{align}
\frac{\partial F}{\partial x}=2x \qquad \frac{\partial F}{\partial y}=2y\\
\frac{dy}{dx}= -\frac{\partial F}{\partial x} / \frac{\partial F}{\partial y}= - \frac{x}{y}\\
\end{align}
$$

## 1.6.2 Example (implicit differentiation of x,y,z)

Given $F(x,y,z)=0$ find $\frac{\partial z}{\partial x}$ and $\frac{\partial z}{\partial y}$

$$
\begin{align}
F(x,y,z)=F(x,y,z(x,y))=0\\
\frac{\partial F}{\partial x}+\frac{\partial F}{\partial z} \left( \frac{\partial z}{\partial x} \right)
_y = 0 \Rightarrow \left( \frac{\partial z}{\partial x} \right)_y=-\frac{\partial F}{\partial x} / \frac{\partial F}{\partial z} \\
\frac{\partial F}{\partial y}+\frac{\partial F}{\partial z} \left( \frac{\partial z}{\partial y} \right)
_y = 0 \Rightarrow \left( \frac{\partial z}{\partial y} \right)_y=-\frac{\partial F}{\partial y} / \frac{\partial F}{\partial z} \\
\end{align}
$$

## 1.6.3 Theorem (implicit function theorem)
see lecture notes for examle of 4 variables

Given a system of $m$ equations $f_i (x_1, \dots, x_n, y_1, \dots, y_m)=0$ ($F(x,y)=0)$) find $\frac{\partial g}{\partial x_j}(x)$

$$
\frac{\partial g}{\partial x_j}(x)=-\left[J_{f,y}(x,g(x)) \right]^{-1}_{m \times m} \left[ \frac{\partial f}{\partial x_j}(x,g(x)) \right] _{m \times 1}
$$

![[Pasted image 20210223220747.png]]

